theories/VLSM/Core/VLSMProjections.v
@@ -1468,7 +1468,7 @@ Definition VLSM_full_projection_finite_valid_trace
 to lift to VLSM full projections the generic results proved about VLSM projections.
 *)
 Lemma VLSM_full_projection_is_projection
-  : VLSM_projection X Y (fun l => Some (label_project l)) state_project.
+  : VLSM_projection X Y (Some ∘ label_project) state_project.
 Proof.
   split.
   - apply VLSM_full_projection_projection_type.
@@ -3298,3 +3298,57 @@ Proof.
 Qed.
 
 End same_VLSM_full_projection.
+
+Section VLSM_projection_composition.
+
+Context
+  {message}
+  [X Y Z : VLSM message]
+  `(HXY : VLSM_projection X Y xy_label xy_state)
+  `(HYZ : VLSM_projection Y Z yz_label yz_state)
+  .
+
+Lemma pre_VLSM_projection_composition_transition_item_project
+  : pre_VLSM_projection_transition_item_project (type X) (type Z)
+      (mbind yz_label ∘ xy_label) (yz_state ∘ xy_state)
+      =
+    mbind (pre_VLSM_projection_transition_item_project (type Y) (type Z) yz_label yz_state)
+      ∘ (pre_VLSM_projection_transition_item_project (type X) (type Y) xy_label xy_state).
+Proof.
+  extensionality item; destruct item; cbn.
+  unfold pre_VLSM_projection_transition_item_project; cbn.
+  destruct (xy_label l) as [lY|]; reflexivity.
+Qed.
+
+Lemma pre_VLSM_projection_composition_finite_trace_project
+  : pre_VLSM_projection_finite_trace_project (type X) (type Z)
+      (mbind yz_label ∘ xy_label) (yz_state ∘ xy_state)
+      =
+    pre_VLSM_projection_finite_trace_project (type Y) (type Z) yz_label yz_state
+      ∘ pre_VLSM_projection_finite_trace_project (type X) (type Y) xy_label xy_state.
+Proof.
+  unfold pre_VLSM_projection_finite_trace_project.
+  setoid_rewrite pre_VLSM_projection_composition_transition_item_project.
+  setoid_rewrite map_option_comp_bind.
+  reflexivity.
+Qed.
+
+Lemma VLSM_projection_composition
+  : VLSM_projection X Z (mbind yz_label ∘ xy_label) (yz_state ∘ xy_state).
+Proof.
+  constructor; [constructor|]; intros sX trX HtrX
+  ; replace (pre_VLSM_projection_finite_trace_project _ _ _ _)
+      with 
+      ((pre_VLSM_projection_finite_trace_project (type Y) (type Z) yz_label yz_state
+      ∘ pre_VLSM_projection_finite_trace_project (type X) (type Y) xy_label xy_state))
+      by (symmetry; apply pre_VLSM_projection_composition_finite_trace_project).
+  - unfold compose.
+    erewrite final_state_project; [|eapply projection_type; eassumption|assumption].
+    eapply final_state_project; [apply projection_type; assumption|].
+    apply VLSM_projection_finite_valid_trace_from with (Hsimul := HXY); assumption.
+  - apply VLSM_projection_finite_valid_trace with (Hsimul := HYZ),
+      VLSM_projection_finite_valid_trace with (Hsimul := HXY).
+    assumption.
+Qed.
+
+End VLSM_projection_composition.
